examples/low-level/example1.fst
@@ -1,0 +1,28 @@
+(*--build-config
+    options:--admit_fsi Set;
+    variables:LIB=../../lib;
+    other-files:$LIB/ext.fst $LIB/set.fsi $LIB/heap.fst $LIB/st.fst $LIB/list.fst stack.fst listset.fst st3.fst
+  --*)
+module Example1
+open StructuredMem
+open Heap
+open Stack
+open Set
+open Prims
+open List
+open ListSet
+
+(*
+val helloWorld : unit -> SST unit  (fun m -> True) (fun m0 a m1 -> True)
+let helloWorld () = let x= halloc 0 in return ()
+*)
+
+(*a good aspect of the current formulation is that the heap/stack difference
+only matters at the time of allocation. Functions like increment can be
+defined without without bothering about that distinction*)
+
+(*
+val increment : (ref int) -> SST unit  (fun m -> True) (fun m0 a m1 -> True)
+let increment r =  (newStackFrame ())
+What is wrong with this?
+*)
